day-4/aeneas/refs.md
@@ -1,7 +1,0 @@
-# Install
-
-# Algos
-- max in list
-- bubble sort
-
-# CSLib
